SSA/Experimental/Bits/MultiWidth/GoodFSM.lean
@@ -11,112 +11,599 @@ import Lean
 
 namespace MultiWidth
 
-instance : HAnd (FSM α) (FSM α) (FSM α) where
-  hAnd := composeBinaryAux' FSM.and
-
-instance : HOr (FSM α) (FSM α) (FSM α) where
-  hOr := composeBinaryAux' FSM.or
-
-instance : HXor (FSM α) (FSM α) (FSM α) where
-  hXor := composeBinaryAux' FSM.xor
-
-instance : Complement (FSM α) where
-  complement := composeUnaryAux FSM.not
-
 
 -- build an FSM whose output is unary, and is 1 in the beginning, and becomes 0
 -- forever after.
 -- TODO: I am pretty sure we can just do this with binary encodings as well?
-def mkWidthFSM (wcard : Nat) (tcard : Nat) (w : Nondep.WidthExpr) : (NatFSM wcard tcard w) :=
+def mkWidthFSM (wcard : Nat) (tcard : Nat) (w : Nondep.WidthExpr) :
+    (NatFSM wcard tcard w) :=
   if h : w.toNat < wcard then
-    { toFsm := composeUnaryAux FSM.scanAnd (FSM.var' (StateSpace.widthVar ⟨w.toNat, h⟩)) }
-  else 
-    { toFsm := FSM.zero.map Fin.elim0 } -- default, should not be used.
+    { toFsm :=
+      -- composeUnaryAux FSM.scanAnd (FSM.var' (StateSpace.widthVar ⟨w.toNat, h⟩))
+      (FSM.var' (StateSpace.widthVar ⟨w.toNat, h⟩))
+    }
+  else
+    { toFsm := FSM.zero' } -- default, should not be used.
 
+
+def IsGoodNatFSM_mkWidthFSM {wcard : Nat} (tcard : Nat) (w : WidthExpr wcard) :
+    HNatFSMToBitstream (mkWidthFSM wcard tcard (.ofDep w)) where
+  heq := by
+    intros wenv fsmEnv henv
+    induction w
+    case var v =>
+      simp [mkWidthFSM]
+      have ⟨henv⟩ := henv
+      rw [henv]
+
+
+/--
+Build an FSM taking inputs 'x' and 'w'.
+Produce the bit 'x[i]' as long as 'w = 1'.
+Once 'w = 0', produce the last value 'x[`last index where w = 1`]
+Otherwise, return if we have found a '1' so far.
+-/
+def fsmMsbAux : FSM Bool where
+  -- when w = 1, store into 'x'.
+  α := Unit
+  initCarry := fun () => false
+  outputCirc :=
+    let s : Circuit (Unit ⊕ (Bool)) := Circuit.var (positive := true) (.inl ())
+    let x : Circuit (Unit ⊕ (Bool)) := Circuit.var (positive := true) (.inr false)
+    let w : Circuit (Unit ⊕ (Bool))  := Circuit.var (positive := true) (.inr true)
+    Circuit.ite w -- if still inside width
+    x -- then update state bit to be 'x'.
+    s -- else return 's'.
+  nextStateCirc := fun () =>
+    let s : Circuit (Unit ⊕ (Bool)) := Circuit.var (positive := true) (.inl ())
+    let x : Circuit (Unit ⊕ (Bool)) := Circuit.var (positive := true) (.inr false)
+    let w : Circuit (Unit ⊕ (Bool)) := Circuit.var (positive := true) (.inr true)
+    -- as long as the width is not exceeded, store into the width.
+    Circuit.ite w -- if w
+      x -- then x
+      s  -- else s
+
+/--
+the MSB finite state machine
+returns the 'msb' upto the current width.
+-/
+def fsmMsb (x w : FSM α) : FSM α :=
+  composeBinaryAux' (FSM.latchImmediate false) (qfalse := x) (qtrue := w)
+
+@[simp]
+theorem eval_fsmMsb_eq {wenv : WidthExpr.Env wcard}
+    {fsmEnv : StateSpace wcard tcard → BitStream}
+    {tctx : Term.Ctx wcard tcard}
+    (tenv : Term.Ctx.Env tctx wenv)
+    (w : WidthExpr wcard)
+    (x : Term tctx w)
+    (xfsm : TermFSM wcard tcard (.ofDep x))
+    (hxfsm : HTermFSMToBitStream xfsm)
+    (wfsm : NatFSM wcard tcard (.ofDep w))
+    (hwfsm : HNatFSMToBitstream wfsm)
+    (htenv : HTermEnv fsmEnv tenv) :
+    (fsmMsb xfsm.toFsm wfsm.toFsm).eval fsmEnv = (fun i =>
+      BitStream.ofBitVecZextMsb (x.toBV tenv) (min i (w.toNat wenv))) := by
+  simp [fsmMsb]
+  have wfsmEval := hwfsm.heq (henv := htenv.toHWidthEnv)
+  have tfsmEval := hxfsm.heq (henv := htenv)
+  ext i
+  rcases i with rfl | i
+  · simp
+    intros hxFsmEq
+    simp [tfsmEval]
+  · simp
+    rw [tfsmEval, wfsmEval]
+    simp
+    induction i
+    case zero =>
+      simp
+      by_cases hw : 1 ≤ w.toNat wenv
+      · simp [hw]
+      · simp at hw
+        simp [hw]
+    case succ i hi =>
+      simp
+      by_cases hxiSucc : (Term.toBV tenv x).getLsbD (i + 1) = true
+      · simp [hxiSucc]
+        by_cases hiwLe : i + 1 + 1  ≤ w.toNat wenv
+        · simp [hiwLe]
+          simp [hxiSucc]
+        · simp [hiwLe]
+          simp at hiwLe
+          have hiwLt := BitVec.lt_of_getLsbD hxiSucc
+          omega
+      · simp at hxiSucc
+        simp [hxiSucc]
+        rw [hi]
+        clear hi
+        generalize hbv : (Term.toBV tenv x) = bv
+        rw [hbv] at hxiSucc
+        by_cases hiSucc : i + 1 ≤ w.toNat wenv
+        · simp [hiSucc]
+          by_cases hiSuccSucc : i + 1 + 1 ≤ w.toNat wenv
+          · simp [hiSuccSucc]
+            rw [hxiSucc]
+          · simp at hiSuccSucc
+            have hwEq : w.toNat wenv = i + 1 := by omega
+            simp [hwEq]
+        · simp at hiSucc
+          simp [show ¬ i + 1 + 1 ≤ w.toNat wenv by omega]
+          simp [show min (i + 1) (w.toNat wenv) = w.toNat wenv by omega]
+          simp [show min (i + 1 + 1) (w.toNat wenv) = w.toNat wenv by omega]
+
+
+-- | Found a cuter expression for 'getLsbD_signExtend'.
+theorem getLsbD_signExtend_eq {wold : Nat} (x : BitVec wold) {wnew : Nat} :
+  (x.signExtend wnew).getLsbD i =
+    (x.getLsbD (min i (wold - 1)) && decide (i < wnew))
+      := by
+  simp [BitVec.getLsbD_signExtend]
+  rw [BitVec.msb_eq_getLsbD_last]
+  by_cases hnew : i < wnew
+  · simp [hnew]
+    by_cases hi : i < wold
+    · simp [hi]
+      simp [show min i (wold - 1) = i by omega]
+    · simp [hi]
+      simp [show min i (wold - 1) = wold - 1 by omega]
+  · simp [hnew]
+
+def fsmSext (x wold wnew : FSM α) : FSM α :=
+  (fsmMsb x wold) &&& wnew
+
+def fsmUnaryMax (a b : FSM arity) : FSM arity :=
+  composeBinaryAux' FSM.or a b
+
+@[simp]
+theorem eval_fsmUnaryMax_eq_decide
+  (a : NatFSM wcard tcard (.ofDep v))
+  (b : NatFSM wcard tcard (.ofDep w))
+  {wenv : WidthExpr.Env wcard}
+  {fsmEnv : StateSpace wcard tcard → BitStream}
+  (henv : HWidthEnv fsmEnv wenv)
+  (ha : HNatFSMToBitstream a) (hb : HNatFSMToBitstream b) :
+  ((fsmUnaryMax a.toFsm b.toFsm).eval fsmEnv) i =
+    (i ≤ (max (v.toNat wenv) (w.toNat wenv))) := by
+  simp only [fsmUnaryMax, composeBinaryAux'_eval, eq_iff_iff]
+  rw [ha.heq (henv := henv)]
+  rw [hb.heq (henv := henv)]
+  simp
+
+def fsmUnaryMin (a b : FSM arity) : FSM arity :=
+  composeBinaryAux' FSM.and a b
+
+/-- compute the 'min' of two FSMs. -/
+@[simp]
+theorem eval_fsmUnaryMin_eq_decide
+  (a : NatFSM wcard tcard (.ofDep v))
+  (b : NatFSM wcard tcard (.ofDep w))
+  {wenv : WidthExpr.Env wcard}
+  {fsmEnv : StateSpace wcard tcard → BitStream}
+  (henv : HWidthEnv fsmEnv wenv)
+  (ha : HNatFSMToBitstream a) (hb : HNatFSMToBitstream b) :
+  ((fsmUnaryMin a.toFsm b.toFsm).eval fsmEnv) i =
+    (i ≤ (min (v.toNat wenv) (w.toNat wenv))) := by
+  simp only [fsmUnaryMin, composeBinaryAux'_eval, _root_.FSM.eval_and, cond_true, cond_false,
+    BitStream.and_eq, Bool.and_eq_true, le_inf_iff, eq_iff_iff]
+  rw [ha.heq (henv := henv)]
+  rw [hb.heq (henv := henv)]
+  simp
+
+/-- increment a unary number by a known constant 'k'. -/
+def fsmUnaryIncrK (k : Nat) (fsm : FSM α) : FSM α :=
+  match k with
+  | 0 => fsm
+  | k + 1 => composeUnaryAux (FSM.ls true) (fsmUnaryIncrK k fsm)
+
+theorem eval_fsmUnaryIncrK_eq_decide
+  (a : NatFSM wcard tcard (.ofDep v))
+  {wenv : WidthExpr.Env wcard}
+  {fsmEnv : StateSpace wcard tcard → BitStream}
+  (henv : HWidthEnv fsmEnv wenv)
+  (ha : HNatFSMToBitstream a) :
+  ((fsmUnaryIncrK k a.toFsm).eval fsmEnv) = fun i =>
+  decide (i ≤ (v.toNat wenv) + k) := by
+  induction k
+  case zero =>
+    simp [fsmUnaryIncrK]
+    rw [ha.heq (henv := henv)]
+  case succ k ih =>
+    simp [fsmUnaryIncrK]
+    rw [ih]
+    ext i
+    rcases i with rfl | i
+    · simp only [BitStream.concat_zero, zero_le, decide_true]
+    · simp only [BitStream.concat_succ, decide_eq_decide]
+      omega
 
 -- when we compute 'a - b', if the borrow bit is zero,
 -- then we know that 'a' is greater than or equal to 'b'.
 -- if the borrow bit is one, then we know that 'a' is less than 'b'.
--- a: 0 <= b: 0 = 1
--- a: 0 <= b: 1 = 1
--- a: 1 <= b: 0 = 0
--- a: 1 <= b: 1 = 1
-def fsmUltUnary (a : FSM α) (b : FSM α) : FSM α :=
-  a ||| ~~~ b
+-- a ≤ b ↔ b[i] = 0 → a[i] = 0
+-- if b = 1, we are done.
+-- Otherwise, if b=0,then a=0
+
+-- alternatively, a[i] = 1 → b[i] = 1.
+-- if a is high, then b must be high for it to be ≤.
+def fsmUnaryUle (a : FSM arity) (b : FSM arity) : FSM arity :=
+ composeUnaryAux FSM.scanAnd (b ||| ~~~ a)
+
+theorem eval_fsmUnaryUle_eq_decide
+    (a : NatFSM wcard tcard (.ofDep v))
+    (b : NatFSM wcard tcard (.ofDep w))
+    {wenv : WidthExpr.Env wcard}
+    {fsmEnv : StateSpace wcard tcard → BitStream}
+    (henv : HWidthEnv fsmEnv wenv)
+    (ha : HNatFSMToBitstream a) (hb : HNatFSMToBitstream b) :
+    ((fsmUnaryUle a.toFsm b.toFsm).eval fsmEnv) i =
+    decide (min i (v.toNat wenv) ≤ min i (w.toNat wenv)) := by
+  simp [fsmUnaryUle]
+  rw [ha.heq (henv := henv)]
+  rw [hb.heq (henv := henv)]
+  induction w generalizing v
+  case var w =>
+    induction v
+    case var v =>
+      simp [BitStream.scanAnd_eq_decide]
+      by_cases hiv : i ≤ wenv v
+      case pos =>
+        by_cases hiw : i ≤ wenv w
+        case pos =>
+          simp [hiw]
+          intros j
+          omega
+        case neg =>
+          simp [hiw]
+          by_cases hvw : wenv v ≤ wenv w
+          case pos =>
+            simp [hvw]
+            intros j
+            omega
+          case neg =>
+            simp [hvw]
+            exists i
+            omega
+      case neg =>
+        by_cases hiw : i ≤ wenv w
+        case pos =>
+          simp [hiw]
+          omega
+        case neg =>
+          simp [hiw]
+          by_cases hvw : wenv v ≤ wenv w
+          case pos =>
+            simp [hvw]
+            omega
+          case neg =>
+            simp [hvw]
+            exists (wenv v)
+            omega
+
+@[simp]
+theorem eval_fsmUnaryUle_eq_lt_or_decide
+    (a : NatFSM wcard tcard (.ofDep v))
+    (b : NatFSM wcard tcard (.ofDep w))
+    {wenv : WidthExpr.Env wcard}
+    {fsmEnv : StateSpace wcard tcard → BitStream}
+    (henv : HWidthEnv fsmEnv wenv)
+    (ha : HNatFSMToBitstream a) (hb : HNatFSMToBitstream b) :
+    ((fsmUnaryUle a.toFsm b.toFsm).eval fsmEnv) i =
+    decide (i ≤ min (v.toNat wenv) (w.toNat wenv) ∨ (v.toNat wenv) ≤ (w.toNat wenv)) := by
+  rw [eval_fsmUnaryUle_eq_decide (wenv := wenv) (henv := henv) (ha := ha) (hb := hb)]
+  simp
+  by_cases hiv : i ≤ v.toNat wenv
+  · simp [hiv]
+  · simp [hiv]
+    omega
+/--
+info: 'MultiWidth.eval_fsmUnaryUle_eq_decide' depends on axioms: [propext, Classical.choice, Quot.sound]
+-/
+#guard_msgs in #print axioms eval_fsmUnaryUle_eq_decide
 
 -- returns 1 if a is equal to b.
-def fsmEqBitwise (a : FSM α) (b : FSM α) : FSM α :=
-  composeUnaryAux FSM.scanAnd <| composeBinaryAux' FSM.nxor a  b
+def fsmEqUnaryUpto (a : FSM arity) (b : FSM arity) : FSM arity :=
+  composeUnaryAux FSM.scanAnd (composeBinaryAux' FSM.nxor a b)
 
--- returns 1 if a is less than or equal to b.
-def fsmUleUnary (a : FSM α) (b : FSM α) : FSM α :=
-  (fsmUltUnary a b) &&& (fsmEqBitwise a b)
+@[simp]
+private theorem min_eq_of_not_le {a b : Nat} (hab : ¬ a ≤ b) : min a b = b := by
+  omega
 
--- | if 'cond' is true, then return 't', otherwise return 'e'.
-def ite (cond : FSM α) (t : FSM α) (e : FSM α) : FSM α :=
-  (cond &&& t) ||| (~~~ cond &&& e)
+@[simp]
+private theorem min_eq_of_not_le' {a b : Nat} (hab : ¬ a ≤ b) : min b a = b := by
+  omega
 
-def fsmZext (a wold wnew : FSM (StateSpace wcard tcard))
+@[simp]
+theorem eval_FsmEqUpto_eq_decide
+    (a : NatFSM wcard tcard (.ofDep v))
+    (b : NatFSM wcard tcard (.ofDep w))
+    {wenv : WidthExpr.Env wcard}
+    {fsmEnv : StateSpace wcard tcard → BitStream}
+    (henv : HWidthEnv fsmEnv wenv)
+    (ha : HNatFSMToBitstream a) (hb : HNatFSMToBitstream b) :
+    ((fsmEqUnaryUpto a.toFsm b.toFsm).eval fsmEnv) i =
+    decide (min i (v.toNat wenv) = min i (w.toNat wenv)) := by
+  simp [fsmEqUnaryUpto]
+  rw [ha.heq (henv := henv)]
+  rw [hb.heq (henv := henv)]
+  induction w generalizing v
+  case var w =>
+    induction v
+    case var v =>
+      simp [BitStream.scanAnd_eq_decide]
+      constructor
+      · intros hi
+        -- | think about what the heck this is saying.
+        by_cases hiv : wenv v ≤ i
+        · have hiv' := hi (wenv v) hiv
+          have := hiv'.mp (by simp)
+          simp [hiv]
+          by_cases hiw : wenv w ≤ i
+          · simp [hiw]
+            have hiw' := hi (wenv w) hiw
+            have := hiw'.mpr (by simp)
+            omega
+          · simp [hiw]
+            have hiv' := hi i (by simp) |>.mpr (by omega)
+            omega
+        · simp [hiv]
+          apply hi .. |>.mp <;> omega
+      · intros hivw j hj
+        omega
+
+@[simp]
+theorem eval_FsmEqUpto_eq_decide'
+    (a : NatFSM wcard tcard (.ofDep v))
+    (b : NatFSM wcard tcard (.ofDep w))
+    {wenv : WidthExpr.Env wcard}
+    {fsmEnv : StateSpace wcard tcard → BitStream}
+    (henv : HWidthEnv fsmEnv wenv)
+    (ha : HNatFSMToBitstream a) (hb : HNatFSMToBitstream b) :
+    ((fsmEqUnaryUpto a.toFsm b.toFsm).eval fsmEnv) = fun i =>
+    decide (min i (v.toNat wenv) = min i (w.toNat wenv)) := by
+  ext i
+  rw [eval_FsmEqUpto_eq_decide (henv := henv) (ha := ha) (hb := hb)]
+
+private theorem decide_eq_eq_decide_iff_decide {P Q : Prop}
+  [Decidable P] [Decidable Q] :
+  (decide P = decide Q) = decide (P ↔ Q) := by
+  simp
+
+private theorem not_decide_eq_decide_lnot {P : Prop}
+  [Decidable P] :
+    (!(decide P)) = (decide (¬ P)) := by simp
+
+private theorem decide_and_decide_eq_decide {P Q : Prop}
+  [Decidable P] [Decidable Q] :
+  (decide P && decide Q) = decide (P ∧ Q) := by
+  simp
+
+private theorem decide_or_decide_eq_decide {P Q : Prop}
+  [Decidable P] [Decidable Q] :
+  (decide P || decide Q) = decide (P ∨ Q) := by
+  simp
+
+/-- returns 1 if a is not equal to b. -/
+def fsmUnaryNeqUpto (a b : FSM arity) : FSM arity :=
+  composeUnaryAux FSM.scanOr (a ^^^ b)
+
+theorem neq_of_min_neq_min {i v w : Nat} (hivw : ¬ min i v = min i w ) :
+  (v ≠ w) := by
+  by_cases hiv : i < v
+  · simp [hiv] at hivw ⊢
+    omega
+  · simp at hiv; simp [hiv] at hivw
+    by_cases hiw : i < w
+    · simp [hiw] at hivw
+      omega
+    · simp at hiw; simp [hiw] at hivw
+      omega
+
+@[simp]
+theorem eval_fsmUnaryNeqUpto_eq_decide
+    (a : NatFSM wcard tcard (.ofDep v))
+    (b : NatFSM wcard tcard (.ofDep w))
+    {wenv : WidthExpr.Env wcard}
+    {fsmEnv : StateSpace wcard tcard → BitStream}
+    (henv : HWidthEnv fsmEnv wenv)
+    (ha : HNatFSMToBitstream a) (hb : HNatFSMToBitstream b) :
+    ((fsmUnaryNeqUpto a.toFsm b.toFsm).eval fsmEnv) i =
+    (decide (min i (v.toNat wenv) ≠ min i (w.toNat wenv))) := by
+  simp [fsmUnaryNeqUpto]
+  rw [ha.heq (henv := henv)]
+  rw [hb.heq (henv := henv)]
+  induction w generalizing v
+  case var w =>
+    induction v
+    case var v =>
+      simp [BitStream.scanOr_eq_decide]
+      rw [not_decide_eq_decide_lnot]
+      rw [decide_eq_eq_decide_iff_decide]
+      rw [decide_eq_true_iff]
+      constructor
+      · intros hi
+        obtain ⟨j, hj₁, hj₂⟩ := hi
+        by_cases hiv : wenv v < i
+        · simp only [not_le, hiv, min_eq_of_not_le]
+          omega
+        · simp only [not_lt] at hiv
+          simp only [hiv, inf_of_le_left, left_eq_inf, not_le]
+          omega
+      · intros hivw
+        simp only [not_iff, not_le]
+        by_cases hiv : i < (wenv v)
+        · simp only [not_le, hiv, min_eq_of_not_le', left_eq_inf] at hivw ⊢
+          exists i
+          omega
+        · simp only [not_lt] at hiv; simp [hiv] at hivw
+          by_cases hiw : i < (wenv w)
+          · simp only [not_le, hiw, min_eq_of_not_le'] at hivw
+            have hiv' : (wenv v) ≤ i := by omega
+            exists i
+            omega
+          · simp only [not_lt] at hiw; simp [hiw] at hivw
+            by_cases hvw : wenv v < wenv w
+            · exists (wenv w)
+              simp only [le_refl, iff_true]
+              omega
+            · simp only [not_lt] at hvw
+              exists (wenv v)
+              omega
+
+
+def fsmUltUnary (a b : FSM arity) : FSM arity :=
+  composeBinaryAux' FSM.and (fsmUnaryUle a b) (fsmUnaryNeqUpto a b)
+
+theorem eval_fsmUltUnary_eq_decide
+    (a : NatFSM wcard tcard (.ofDep v))
+    (b : NatFSM wcard tcard (.ofDep w))
+    {wenv : WidthExpr.Env wcard}
+    {fsmEnv : StateSpace wcard tcard → BitStream}
+    (henv : HWidthEnv fsmEnv wenv)
+    (ha : HNatFSMToBitstream a) (hb : HNatFSMToBitstream b) :
+    ((fsmUltUnary a.toFsm b.toFsm).eval fsmEnv) i =
+   (decide (min i (v.toNat wenv) < min i (w.toNat wenv))) := by
+  simp [fsmUltUnary]
+  rw [eval_fsmUnaryUle_eq_lt_or_decide (wenv := wenv) (henv := henv) (ha := ha) (hb := hb)]
+  rw [eval_fsmUnaryNeqUpto_eq_decide (wenv := wenv) (henv := henv) (ha := ha) (hb := hb)]
+  simp
+  generalize v.toNat wenv = v'
+  generalize w.toNat wenv = w'
+  simp only [not_decide_eq_decide_lnot,
+    decide_and_decide_eq_decide,
+    decide_or_decide_eq_decide, decide_eq_decide]
+  omega
+
+private theorem BitVec.getLsbD_zeroExtend_eq_getLsbD (x : BitVec wold) (wnew : Nat) :
+    (x.zeroExtend wnew).getLsbD i = ((x.getLsbD i) ∧ (i ≤ wnew - 1) ∧ (wnew ≠ 0)) := by
+  simp [and_comm]; try omega
+
+/-- this creates an FSM that returns whether 'a ≤ i' -/
+def fsmUnaryIndexUle (a : NatFSM wcard tcard (.ofDep v)) :
+    FSM (StateSpace wcard tcard) :=
+  a.toFsm
+
+@[simp]
+theorem fsmIndexUle_eval_eq
+    (a : NatFSM wcard tcard (.ofDep v))
+    {wenv : WidthExpr.Env wcard}
+    {fsmEnv : StateSpace wcard tcard → BitStream}
+    (henv : HWidthEnv fsmEnv wenv)
+    (ha : HNatFSMToBitstream a) :
+    (fsmUnaryIndexUle a).eval fsmEnv i =
+    decide (i ≤ v.toNat wenv) := by
+  rw [fsmUnaryIndexUle]
+  rw [ha.heq (henv := henv)]
+
+def fsmZext (nFsm wnewfsm : FSM (StateSpace wcard tcard))
     : FSM (StateSpace wcard tcard) :=
-  ite (fsmUleUnary wold wnew) a (FSM.zero.map Fin.elim0)
-
-/-- The inputs given to the sext fsm. -/
-inductive fsmSext.inputs
-| a
-| a0
-| wold
-| wnew
-
-def fsmSext.inputs.toFin : fsmSext.inputs → Fin 4
-| .a => 0
-| .a0 => 1
-| .wold => 2
-| .wnew => 3
+  nFsm &&& (wnewfsm)
 
 
-def fsmSext (a wold wnew : FSM (StateSpace wcard tcard))
-    : FSM (StateSpace wcard tcard) :=
-    ite (fsmUleUnary wnew wold)
-      /- wnew ≤ wold, so it's the same as zext. -/
-      (fsmZext a wold wnew)
-      /- wnew > wold. -/
-    (composeQuaternaryAux'
-      (composer.map fsmSext.inputs.toFin)
-      a
-      (composeUnaryAux (FSM.ls false) a)
-      wold
-      wnew)
-  where
-    -- precondition: wnew > wold.
-    composer : FSM fsmSext.inputs := {
-      α := Unit,
-      initCarry := fun () => false,
-      outputCirc :=
-        .ite (.var true (.inr fsmSext.inputs.wold)) -- i ≤ wold < wnew
-          (.var true (.inr fsmSext.inputs.a)) -- return the bit of a.
-          -- else: wold < i ≤ wnew
-          (.ite (.var true (.inr fsmSext.inputs.wnew))
-            (.var true (.inl ())) -- return our state bit.
-            -- else: wnew < i.
-            .fals
-          )
-      nextStateCirc :=
-        /- while we are i ≤ wold, store the bit from a. -/
-        /- otherwise, save the old bit. -/
-        fun () =>
-          .ite (.var true (.inr fsmSext.inputs.wold))
-            (.var true (.inr fsmSext.inputs.a)) -- i ≤ wold
-            (.var true (.inl ())) -- i > wold
-    }
+/-- the fsmZext builds the correct zero-extended FSM. -/
+theorem fsmZext_eval_eq
+    (wnewFsm : NatFSM wcard tcard (.ofDep wnew))
+    {wenv : WidthExpr.Env wcard}
+    {fsmEnv : StateSpace wcard tcard → BitStream}
+    (hwnew : HNatFSMToBitstream wnewFsm)
+    {tctx : Term.Ctx wcard tcard}
+    (tenv : Term.Ctx.Env tctx wenv)
+    (t : Term tctx w)
+    (tFsm : TermFSM wcard tcard (.ofDep t))
+    (ht : HTermFSMToBitStream tFsm)
+    (htenv : HTermEnv fsmEnv tenv) :
+    (fsmZext tFsm.toFsm wnewFsm.toFsm).eval fsmEnv = fun i =>
+      ((BitStream.ofBitVecZextMsb ((Term.zext t wnew).toBV tenv))) i := by
+  ext i
+  rw [fsmZext]
+  simp only [FSM.eval_and', BitStream.and_eq, BitStream.ofBitVecZextMsb_eq_concat_ofBitVecZext]
+  rw [ht.heq (henv := htenv)]
+  rw [hwnew.heq (henv := htenv.toHWidthEnv)]
+  simp
+  rcases i with rfl | i
+  · simp
+  · simp
+    by_cases hi : i < wnew.toNat wenv
+    · simp [hi]
+      intros hval
+      omega
+    · simp [hi]
+      omega
 
+/-- the fsmZext builds the correct zero-extended FSM. -/
+theorem fsmSext_eval_eq
+    (woldFsm : NatFSM wcard tcard (.ofDep wold))
+    (wnewFsm : NatFSM wcard tcard (.ofDep wnew))
+    {wenv : WidthExpr.Env wcard}
+    {fsmEnv : StateSpace wcard tcard → BitStream}
+    (hwnew : HNatFSMToBitstream wnewFsm)
+    (hwold : HNatFSMToBitstream woldFsm)
+    {tctx : Term.Ctx wcard tcard}
+    (tenv : Term.Ctx.Env tctx wenv)
+    (t : Term tctx wold)
+    (tFsm : TermFSM wcard tcard (.ofDep t))
+    (htfsm : HTermFSMToBitStream tFsm)
+    (htenv : HTermEnv fsmEnv tenv) :
+    (fsmSext tFsm.toFsm woldFsm.toFsm  wnewFsm.toFsm).eval fsmEnv = fun i =>
+      ((BitStream.ofBitVecZextMsb ((Term.sext t wnew).toBV tenv))) i := by
+  ext i
+  rw [fsmSext]
+  simp only [FSM.eval_and', BitStream.and_eq,
+    BitStream.ofBitVecZextMsb_eq_concat_ofBitVecZext]
+  rw [hwnew.heq (henv := htenv.toHWidthEnv)]
+  rw [eval_fsmMsb_eq
+        (xfsm := tFsm) (wfsm := woldFsm) (htenv := htenv)
+        (hxfsm := htfsm) (hwfsm := hwold)]
+  simp
+  by_cases hwold : i ≤ wold.toNat wenv
+  · simp [hwold]
+    by_cases hwnew : i ≤ wnew.toNat wenv
+    · simp [hwnew]
+      rcases i with rfl | i
+      · simp
+      · simp [BitVec.getLsbD_signExtend]
+        simp [show i < wnew.toNat wenv by omega]
+        omega
+    · simp [hwnew]
+      rcases i with rfl | i
+      · simp
+      · simp [BitVec.getLsbD_signExtend]
+        omega
+  · simp [hwold]
+    by_cases hwnew : i ≤ wnew.toNat wenv
+    · simp [hwnew]
+      -- TODO: needs fsmMsbAux.
+      rcases i with rfl | i
+      · simp
+        omega
+      · simp
+        simp at hwold
+        rw [getLsbD_signExtend_eq]
+        simp [show min i (wold.toNat wenv - 1) = wold.toNat wenv - 1 by omega]
+        simp [show i < wnew.toNat wenv by omega]
+        have hwold : wold.toNat wenv = 0 ∨ 0 < wold.toNat wenv := by
+          omega
+        rcases hwold with hwold | hwold
+        · simp [hwold]
+        · simp [hwold]
+    · simp [hwnew]
+      rcases i with rfl | w
+      · simp
+      · simp
+        rw [BitVec.getLsbD_signExtend]
+        simp; omega
 
-def mkTermFSM (wcard tcard : Nat) (t : Nondep.Term) : 
+/-- info: 'MultiWidth.fsmSext_eval_eq' depends on axioms: [propext, Classical.choice, Quot.sound] -/
+#guard_msgs in #print axioms fsmSext_eval_eq
+
+def mkTermFSM (wcard tcard : Nat) (t : Nondep.Term) :
     (TermFSM wcard tcard t) :=
   match t with
   | .var v _w =>
     if h : v < tcard then
       {
-      toFsm := composeUnaryAux FSM.scanAnd (FSM.var' (StateSpace.termVar ⟨v, h⟩))
+      -- toFsm := composeUnaryAux FSM.scanAnd (FSM.var' (StateSpace.termVar ⟨v, h⟩))
+      toFsm := (FSM.var' (StateSpace.termVar ⟨v, h⟩))
       }
     else
       { toFsm := FSM.zero.map Fin.elim0 } -- default, should not be ued.
@@ -125,11 +612,11 @@ def mkTermFSM (wcard tcard : Nat) (t : Nondep.Term) :
     let fsmB := mkTermFSM wcard tcard b
     { toFsm := (composeBinaryAux' FSM.add fsmA.toFsm fsmB.toFsm) }
   | .zext a wnew =>
-      let wold := a.width
+      -- let wold := a.width
       let afsm := mkTermFSM wcard tcard a
-      let woldFsm := mkWidthFSM wcard tcard wold
+      -- let woldFsm := mkWidthFSM wcard tcard wold
       let wnewFsm := mkWidthFSM wcard tcard wnew
-      { toFsm := fsmZext afsm.toFsm woldFsm.toFsm wnewFsm.toFsm }
+      { toFsm := fsmZext afsm.toFsm wnewFsm.toFsm }
   | .sext a v =>
     let wold := a.width
     let afsm := mkTermFSM wcard tcard a
@@ -137,25 +624,186 @@ def mkTermFSM (wcard tcard : Nat) (t : Nondep.Term) :
     let vFsm := mkWidthFSM wcard tcard v
     { toFsm := fsmSext afsm.toFsm woldFsm.toFsm vFsm.toFsm }
 
-/-- fSM that returns 1 ifthe predicate is true, and 0 otherwise -/
+axiom AxAdd {P : Prop} : P
+
+def IsGoodTermFSM_mkTermFSM (wcard tcard : Nat) {tctx : Term.Ctx wcard tcard}
+    {wold : WidthExpr wcard}
+    (t : Term tctx wold) :
+    (HTermFSMToBitStream (mkTermFSM wcard tcard (.ofDep t))) := by
+  induction t
+  case var v =>
+    constructor
+    intros wenv tenv fsmEnv htenv
+    obtain htenv_term := htenv.heq_term
+    obtain htenv_width := htenv.heq_width
+    simp only [Nondep.Term.ofDep_var, mkTermFSM,
+      Fin.is_lt, ↓reduceDIte, Fin.eta, FSM.eval_var', htenv_term,
+      BitStream.ofBitVecZextMsb_eq_concat_ofBitVecZext, Term.toBV_var]
+  case add v p q hp hq =>
+    constructor
+    intros wenv tenv fsmEnv htenv
+    simp [Nondep.Term.ofDep, mkTermFSM]
+    ext i
+    rw [hp.heq (henv := htenv)]
+    rw [hq.heq (henv := htenv)]
+    simp only [BitStream.ofBitVecZextMsb_eq_concat_ofBitVecZext]
+    rw [← BitStream.add_eq]
+    rw [BitStream.add]
+    exact AxAdd
+  case zext w' a wnew ha  =>
+    constructor
+    intros wenv tenv fsmEnv htenv
+    simp [Nondep.Term.ofDep, mkTermFSM]
+    let hwnew := IsGoodNatFSM_mkWidthFSM tcard wnew
+    rw [fsmZext_eval_eq (htenv := htenv) (wnew := wnew) (ht := ha) (hwnew := hwnew)]
+    simp
+  case sext wold a wnew ha =>
+    constructor
+    intros wenv tenv fsmEnv htenv
+    let hwold := IsGoodNatFSM_mkWidthFSM tcard wold
+    let hwnew := IsGoodNatFSM_mkWidthFSM tcard wnew
+    simp [Nondep.Term.ofDep, mkTermFSM]
+    -- | TODO: why does this not unify?
+    rw [MultiWidth.Nondep.Term.width_ofDep_eq_ofDep]
+    rw [fsmSext_eval_eq (htenv := htenv) (tenv := tenv)
+      (wold := wold) (wnew := wnew) (t := a) (htfsm := ha)
+      (hwnew := hwnew) (hwold := hwold)]
+    simp
+
+def fsmTermEq {wcard tcard : Nat}
+  {a b : Nondep.Term}
+  (afsm : TermFSM wcard tcard a)
+  (bfsm : TermFSM wcard tcard b)
+  -- (ha : IsGoodTermFSM afsm)
+  -- (hb : IsGoodTermFSM bfsm)
+  : FSM (StateSpace wcard tcard) :=
+    composeUnaryAux FSM.scanAnd
+    (composeBinaryAux' FSM.nxor afsm.toFsm  bfsm.toFsm)
+
+
+-- fSM that returns 1 ifthe predicate is true, and 0 otherwise -/
 def mkPredicateFSMAux (wcard tcard : Nat) (p : Nondep.Predicate) :
   (PredicateFSM wcard tcard p) :=
   match p with
   | .binRel .eq a b =>
     let fsmA := mkTermFSM wcard tcard a
     let fsmB := mkTermFSM wcard tcard b
-    { toFsm := fsmEqBitwise fsmA.toFsm fsmB.toFsm }
+    { toFsm := fsmTermEq fsmA fsmB }
   | .or p q  =>
     let fsmP :=  mkPredicateFSMAux wcard tcard p
     let fsmQ :=  mkPredicateFSMAux wcard tcard q
-    { toFsm := composeUnaryAux FSM.scanAnd (fsmP.toFsm ||| fsmQ.toFsm) }
+    let fsmP := composeUnaryAux FSM.scanAnd fsmP.toFsm
+    let fsmQ := composeUnaryAux FSM.scanAnd fsmQ.toFsm
+    { toFsm := (fsmP ||| fsmQ) }
   | .and p q =>
     let fsmP := mkPredicateFSMAux wcard tcard p
     let fsmQ := mkPredicateFSMAux wcard tcard q
-    { toFsm := composeUnaryAux FSM.scanAnd (fsmP.toFsm &&& fsmQ.toFsm) }
-  | .not p =>
-    let fsmP := mkPredicateFSMAux wcard tcard p
-    { toFsm := composeUnaryAux FSM.scanAnd (~~~ fsmP.toFsm) }
+    { toFsm := (fsmP.toFsm &&& fsmQ.toFsm) }
+
+theorem foo (f g : α → β) (h : f ≠ g) : ∃ x, f x ≠ g x := by
+  exact Function.ne_iff.mp h
+
+def isGoodPredicateFSM_mkPredicateFSMAux {wcard tcard : Nat}
+    {tctx : Term.Ctx wcard tcard}
+    (p : MultiWidth.Predicate tctx) :
+    HPredFSMToBitStream (mkPredicateFSMAux wcard tcard (.ofDep p)) := by
+  induction p
+  case binRel w rel a b =>
+    rcases rel
+    case eq =>
+      constructor
+      intros wenv tenv fsmEnv henv
+      simp [mkPredicateFSMAux, Nondep.Predicate.ofDep]
+      -- fsmTermEqProof starts here.
+      simp [fsmTermEq]
+      have ha := IsGoodTermFSM_mkTermFSM wcard tcard a
+      have hb := IsGoodTermFSM_mkTermFSM wcard tcard b
+      rw [ha.heq (henv := henv)]
+      rw [hb.heq (henv := henv)]
+      simp [Predicate.toProp]
+      constructor
+      · intros h
+        simp at h
+        ext N
+        simp
+        rw [h]
+        rw [BitStream.scanAnd_eq_decide]
+        simp
+      · intros h
+        apply BitVec.eq_of_getLsbD_eq
+        intros i hi
+        have := congrFun h (i + 1)
+        simp at this
+        simp [this]
+  case or p q hp hq =>
+    constructor
+    intros wenv tenv fsmEnv henv
+    simp [mkPredicateFSMAux, Nondep.Predicate.ofDep]
+    simp [Predicate.toProp]
+    rw [hp.heq (henv := henv)]
+    rw [hq.heq (henv := henv)]
+    constructor
+    · intros h
+      ext i
+      simp only [BitStream.or_eq, BitStream.negOne_eq, Bool.or_eq_true]
+      rcases h with h | h
+      · left
+        rw [BitStream.scanAnd_eq_decide]
+        simp
+        intros j hj
+        have := congrFun h j
+        simp at this
+        simp [this]
+      · right
+        rw [BitStream.scanAnd_eq_decide]
+        simp
+        intros j hj
+        have := congrFun h j
+        simp at this
+        simp [this]
+    · intros h
+      by_contra h'
+      simp at h'
+      obtain ⟨h1, h2⟩ := h'
+      have h1 := Function.ne_iff.mp h1
+      have h2 := Function.ne_iff.mp h2
+      obtain ⟨i1, h1⟩ := h1
+      simp at h1
+      obtain ⟨i2, h2⟩ := h2
+      simp at h2
+      have := congrFun h (max i1 i2)
+      simp at this
+      rcases this with this | this
+      · rw [BitStream.scanAnd_eq_decide] at this
+        simp at this
+        specialize this i1 (by omega)
+        simp [this] at h1
+      · rw [BitStream.scanAnd_eq_decide] at this
+        simp at this
+        specialize this i2 (by omega)
+        simp [this] at h2
+  case and p q hp hq =>
+    constructor
+    simp [mkPredicateFSMAux, Nondep.Predicate.ofDep]
+    intros wenv tenv fsmEnv htenv
+    simp [Predicate.toProp]
+    rw [hp.heq (henv := htenv)]
+    rw [hq.heq (henv := htenv)]
+    constructor
+    · intros h
+      obtain ⟨hpfsm, hqfsm⟩ := h
+      simp [hpfsm, hqfsm]
+      ext i; simp
+    · intros h
+      constructor
+      · ext i
+        have := congrFun h i
+        simp at this
+        simp [this]
+      · ext i
+        have := congrFun h i
+        simp at this
+        simp [this]
 
 /-- Negate the FSM so we can decide if zeroes. -/
 def mkPredicateFSMNondep (wcard tcard : Nat) (p : Nondep.Predicate) :
@@ -169,6 +817,15 @@ def mkPredicateFSMDep {wcard tcard : Nat} {tctx : Term.Ctx wcard tcard}
 
 axiom AxGoodFSM {P : Prop} : P
 
+section BitStream2BV
+
+variable
+  {tctx : Term.Ctx wcard tcard}
+    (p : Predicate tctx)
+
+end BitStream2BV
+
+
 
 -- | TODO: rename these namespaces.
 open ReflectVerif BvDecide Std Tactic BVDecide Frontend in
@@ -176,22 +833,40 @@ open ReflectVerif BvDecide Std Tactic BVDecide Frontend in
 then the predicate is satisfied.
 -/
 theorem Predicate.toProp_of_KInductionCircuits
-   {wcard tcard : Nat}
-   (tctx : Term.Ctx wcard tcard)
-   (p : MultiWidth.Predicate tctx)
-   (pNondep : Nondep.Predicate)
-   (_hpNondep : pNondep = (.ofDep p))
-   (fsm : PredicateFSM wcard tcard pNondep)
-   (_hfsm : fsm = mkPredicateFSMNondep wcard tcard pNondep)
-   (n : Nat)
-   (circs : KInductionCircuits fsm.toFsm n)
-   (_hCircs : circs.IsLawful)
-   (sCert : Lean.Elab.Tactic.BVDecide.Frontend.LratCert)
-   (_hs : Circuit.verifyCircuit (circs.mkSafetyCircuit) sCert = true)
-   (indCert : Lean.Elab.Tactic.BVDecide.Frontend.LratCert)
-   (_hind : Circuit.verifyCircuit (circs.mkIndHypCycleBreaking) indCert = true)
-   (wenv : WidthExpr.Env wcard)
-   (tenv : tctx.Env wenv) :
-  p.toProp tenv := by exact AxGoodFSM
+    {wcard tcard : Nat}
+    (tctx : Term.Ctx wcard tcard)
+    (p : MultiWidth.Predicate tctx)
+    (pNondep : Nondep.Predicate)
+    (_hpNondep : pNondep = (.ofDep p))
+    (fsm : PredicateFSM wcard tcard pNondep)
+    (_hfsm : fsm = mkPredicateFSMNondep wcard tcard pNondep)
+    (n : Nat)
+    (circs : KInductionCircuits fsm.toFsm n)
+    (hCircs : circs.IsLawful)
+    (sCert : Lean.Elab.Tactic.BVDecide.Frontend.LratCert)
+    (hs : Circuit.verifyCircuit (circs.mkSafetyCircuit) sCert = true)
+    (indCert : Lean.Elab.Tactic.BVDecide.Frontend.LratCert)
+    (hind : Circuit.verifyCircuit (circs.mkIndHypCycleBreaking) indCert = true)
+    (wenv : WidthExpr.Env wcard)
+    (tenv : tctx.Env wenv) :
+    p.toProp tenv := by
+  have hGoodPredicateFSM := isGoodPredicateFSM_mkPredicateFSMAux p
+  rw [hGoodPredicateFSM.heq (tenv := tenv)
+    (fsmEnv := HTermEnv.mkFsmEnvOfTenv tenv)]
+  · subst _hpNondep _hfsm
+    simp [mkPredicateFSMNondep] at circs
+    apply ReflectVerif.BvDecide.KInductionCircuits.eval_eq_negOne_of_mkIndHypCycleBreaking_eval_eq_false_of_mkSafetyCircuit_eval_eq_false'
+      (circs := circs) (hCircs := hCircs) (envBitstream := (HTermEnv.mkFsmEnvOfTenv tenv))
+      (hSafety := Circuit.eval_eq_false_of_verifyCircuit hs)
+      (hIndHyp := Circuit.eval_eq_false_of_verifyCircuit hind)
+  · simp
+
+/--
+info: 'MultiWidth.Predicate.toProp_of_KInductionCircuits' depends on axioms: [propext,
+ Classical.choice,
+ MultiWidth.AxAdd,
+ Quot.sound]
+-/
+#guard_msgs in #print axioms Predicate.toProp_of_KInductionCircuits
 
 end MultiWidth
